tests/lean/with_cases.lean
@@ -1,0 +1,18 @@
+open tactic
+
+example (p q : Prop) [s₁ : decidable p] [s₂ : decidable q] : true :=
+begin
+  with_cases { cases s₁; cases s₂ },
+  trace_state,
+  all_goals { intros, trivial }
+end
+
+def split (p : Prop) {q : Prop} [decidable p] (pos : p → q) (neg : ¬ p → q) : q :=
+decidable.by_cases pos neg
+
+example (p q : Prop) [decidable p] [decidable q] : true :=
+begin
+  with_cases { apply split p; apply split q; intros hq hp },
+  trace_state,
+  all_goals { intros, trivial }
+end
